theories/s4/interp.v
@@ -1,7 +1,8 @@
 From Coq Require Import ssreflect.
 From stdpp Require Import prelude.
 From bunched.algebra Require Import bi.
-From bunched Require Import seqcalc_s4.
+From bunched Require Import bunches.
+From bunched.s4 Require Import formula seqcalc.
 
 (** * Interpretation of the sequent calculus in an arbitrary BI. *)
 
@@ -19,6 +20,8 @@ Section interp.
   Variable (PROP : bi).
   Variable (box : PROP → PROP).
   Context `{!BiBox PROP box}.
+  Notation bunch := (@bunch formula).
+  Notation bunch_ctx := (@bunch_ctx formula).
 
   Notation "□ A" := (box A) : bi_scope.
 
@@ -44,111 +47,37 @@ Section interp.
     | BOX ϕ => □ (formula_interp ϕ)
     end%I.
 
-  Fixpoint bunch_interp (Δ : bunch) : PROP :=
-    match Δ with
-    | frml ϕ => formula_interp ϕ
-    | top => True
-    | empty => emp
-    | (Δ ,, Δ')%B => bunch_interp Δ ∗ bunch_interp Δ'
-    | (Δ ;, Δ')%B => bunch_interp Δ ∧ bunch_interp Δ'
-    end%I.
+  Notation bunch_interp := (bunch_interp formula_interp).
 
   Lemma bunch_interp_collapse Δ :
-    bunch_interp Δ ≡ formula_interp (collapse Δ).
+    bunch_interp Δ = formula_interp (collapse Δ).
   Proof.
-    induction Δ; simpl; eauto.
-    - by rewrite IHΔ1 IHΔ2.
-    - by rewrite IHΔ1 IHΔ2.
+    induction Δ as [ϕ|sp|sp Δ1 IH1 Δ2 IH2]; try destruct sp; simpl; eauto.
+    - by rewrite IH1 IH2.
+    - by rewrite IH1 IH2.
+  Qed.
+
+  Lemma bunch_interp_box Δ :
+    bunch_interp (BOX <$> Δ) ⊢ □ (bunch_interp Δ).
+  Proof.
+    induction Δ as [ϕ|sp|sp Δ1 IH1 Δ2 IH2]; try destruct sp; simpl; eauto.
+    - apply bi_box_emp.
+    - apply bi_box_true.
+    - rewrite IH1 IH2. apply bi_box_sep.
+    - rewrite IH1 IH2. apply bi_box_conj.
+  Qed.
+
+  Lemma bunch_interp_box_idem (Δ : bunch) :
+    bunch_interp (BOX <$> Δ) ⊢ bunch_interp (BOX <$> (BOX <$> Δ)).
+  Proof.
+    induction Δ as [ϕ|sp|sp Δ1 IH1 Δ2 IH2]; try destruct sp; simpl; eauto.
+    - apply bi_box_idem.
+    - by rewrite IH1 IH2.
+    - by rewrite IH1 IH2.
   Qed.
 
   Definition seq_interp Δ ϕ : Prop :=
     (bunch_interp Δ ⊢ formula_interp ϕ).
-
-  Definition bunch_ctx_item_interp (C : bunch_ctx_item) : PROP → PROP :=
-    λ P, match C with
-         | CtxCommaL Δ => P ∗ bunch_interp Δ
-         | CtxCommaR Δ => bunch_interp Δ ∗ P
-         | CtxSemicL Δ => P ∧ bunch_interp Δ
-         | CtxSemicR Δ => bunch_interp Δ ∧ P
-         end%I.
-
-  Definition bunch_ctx_interp Π : PROP → PROP :=
-    λ P, foldl (flip bunch_ctx_item_interp) P Π.
-
-  Lemma bunch_ctx_interp_cons F Π A :
-    bunch_ctx_interp (F::Π) A = bunch_ctx_interp Π (bunch_ctx_item_interp F A).
-  Proof. reflexivity. Qed.
-
-  Global Instance bunch_ctx_interp_proper Π : Proper ((≡) ==> (≡)) (bunch_ctx_interp Π).
-  Proof.
-    induction Π as [|F Π]=>X Y HXY.
-    - simpl; auto.
-    - simpl.
-      eapply IHΠ.
-      destruct F; solve_proper.
-  Qed.
-
-  Lemma bunch_ctx_interp_decomp Π Δ :
-    bunch_interp (fill Π Δ) ≡ bunch_ctx_interp Π (bunch_interp Δ).
-  Proof.
-    revert Δ. induction Π as [|C Π IH]=>Δ; first by reflexivity.
-    apply bi.equiv_entails_2.
-    - destruct C; simpl; by rewrite IH.
-    - destruct C; simpl; by rewrite IH.
-  Qed.
-
-  Lemma bunch_interp_fill_item_mono (C : bunch_ctx_item) Δ Δ' :
-    (bunch_interp Δ ⊢ bunch_interp Δ') →
-    bunch_interp (fill_item C Δ) ⊢ bunch_interp (fill_item C Δ').
-  Proof.
-    intros H1.
-    induction C as [ ? | ? | ? | ? ]; simpl; by rewrite H1.
-  Qed.
-
-  Lemma bunch_interp_fill_mono Π Δ Δ' :
-    (bunch_interp Δ ⊢ bunch_interp Δ') →
-    bunch_interp (fill Π Δ) ⊢ bunch_interp (fill Π Δ').
-  Proof.
-    revert Δ Δ'.
-    induction Π as [|C Π IH]=> Δ Δ' H1; eauto.
-    simpl. apply IH.
-    by apply bunch_interp_fill_item_mono.
-  Qed.
-
-  Lemma bunch_interp_box Δ :
-    bunch_interp (bunch_map BOX Δ) ⊢ box (bunch_interp Δ).
-  Proof.
-    induction Δ; simpl; eauto.
-    - apply bi_box_true.
-    - apply bi_box_emp.
-    - rewrite IHΔ1 IHΔ2. apply bi_box_sep.
-    - rewrite IHΔ1 IHΔ2. apply bi_box_conj.
-  Qed.
-  Lemma bunch_interp_box_idem Δ :
-    bunch_interp (bunch_map BOX Δ) ⊢ bunch_interp (bunch_map BOX (bunch_map BOX Δ)).
-  Proof.
-    induction Δ; simpl; eauto.
-    - apply bi_box_idem.
-    - by rewrite IHΔ1 IHΔ2.
-    - by rewrite IHΔ1 IHΔ2.
-  Qed.
-
-  Global Instance bunch_interp_proper : Proper ((≡) ==> (≡)) bunch_interp.
-  Proof.
-    intros Δ1 Δ2. induction 1; eauto.
-    - etrans; eassumption.
-    - apply bi.equiv_entails_2.
-      + apply bunch_interp_fill_mono; eauto.
-        by apply bi.equiv_entails_1_1.
-      + apply bunch_interp_fill_mono; eauto.
-        by apply bi.equiv_entails_1_2.
-    - simpl. by rewrite left_id.
-    - simpl. by rewrite comm.
-    - simpl. by rewrite assoc.
-    - simpl. by rewrite left_id.
-    - simpl. by rewrite comm.
-    - simpl. by rewrite assoc.
-  Qed.
 
   Global Instance seq_interp_proper : Proper ((≡) ==> (=) ==> (≡)) seq_interp.
   Proof.
@@ -177,7 +106,7 @@ Section interp.
     - induction C as [|C Π IH]; simpl.
       { apply bi.False_elim. }
       rewrite -IH.
-      destruct C; simpl; apply bunch_interp_fill_mono; simpl.
+      destruct C as [[] ?|  [] ?]; simpl; apply bunch_interp_fill_mono; simpl.
       all: by rewrite ?left_absorb ?right_absorb.
     - apply bi.True_intro.
     - by rewrite IHproves1 IHproves2.
@@ -187,9 +116,9 @@ Section interp.
       revert ϕ ψ.
       induction Π as [|F Π] => /= ϕ ψ IH1 IH2.
       { apply bi.or_elim; eauto. }
-      destruct F; simpl; simpl in IH1, IH2;
+      destruct F as [[] ? IH1|[] ? IH2]; simpl; simpl in IH1, IH2;
       rewrite bunch_ctx_interp_decomp;
-      cbn[bunch_interp formula_interp].
+      cbn[sep_interp bunch_interp formula_interp].
       + rewrite bi.sep_or_r.
         unfold seq_interp in *.
         etrans.
@@ -203,10 +132,10 @@ Section interp.
         rewrite bunch_ctx_interp_decomp.
         cbn[bunch_interp formula_interp].
         by rewrite bunch_interp_collapse.
-      + rewrite bi.sep_or_l.
+      + rewrite bi.and_or_r.
         unfold seq_interp in *.
         etrans.
-        2:{ eapply (IHΠ (SEP (collapse Δ1) ϕ) (SEP (collapse Δ1) ψ)).
+        2:{ eapply (IHΠ (CONJ ϕ (collapse Δ2)) (CONJ ψ (collapse Δ2))).
             - rewrite -IH1.
               apply bunch_interp_fill_mono; simpl.
               by rewrite bunch_interp_collapse.
@@ -216,10 +145,10 @@ Section interp.
         rewrite bunch_ctx_interp_decomp.
         cbn[bunch_interp formula_interp].
         by rewrite bunch_interp_collapse.
-      + rewrite bi.and_or_r.
+      + rewrite bi.sep_or_l.
         unfold seq_interp in *.
         etrans.
-        2:{ eapply (IHΠ (CONJ ϕ (collapse Δ2)) (CONJ ψ (collapse Δ2))).
+        2:{ eapply (IHΠ (SEP (collapse Δ1) ϕ) (SEP (collapse Δ1) ψ)).
             - rewrite -IH1.
               apply bunch_interp_fill_mono; simpl.
               by rewrite bunch_interp_collapse.
