theories/s4/seqcalc_height.v
@@ -1,29 +1,26 @@
 (* Sequent calculus with upper bounds on proof size.
    Useful for doing induction on.
 
-   The main purpose this file is to provide the inversion lemmas (see the bottom part of the file).
+   The main purpose this file is to provide the inversion lemmas (at the very bottom of the file).
  *)
 From Coq Require Import ssreflect.
 From stdpp Require Import prelude.
 From bunched.algebra Require Import bi.
-From bunched Require Import seqcalc bunch_decomp prelude.lists.
+From bunched.s4 Require Import formula seqcalc.
 
 Reserved Notation "P ⊢ᴮ{ n } Q" (at level 99, n, Q at level 200, right associativity).
 Reserved Notation "Δ =?{ n } Δ'" (at level 99, n at level 200).
 
-Module SeqcalcHeight(R : ANALYTIC_STRUCT_EXT).
-  Import R.
-  Module S := Seqcalc(R).
-  Import S.
-
+Section SeqcalcHeight.
+  Notation bunch := (@bunch formula).
   Implicit Type Δ : bunch.
   Implicit Type ψ ϕ : formula.
 
   (** ** Alternative formulation of bunch equivalences *)
   Inductive bunch_equiv : bunch → bunch → Prop :=
-  | BE_cong C Δ1 Δ2 :
+  | BE_cong Π Δ1 Δ2 :
       Δ1 =? Δ2 →
-      fill C Δ1 =? fill C Δ2
+      fill Π Δ1 =? fill Π Δ2
   | BE_comma_unit_l Δ :
       (∅ₘ ,, Δ)%B =? Δ
   | BE_comma_comm Δ1 Δ2 :
@@ -53,13 +50,13 @@ Module SeqcalcHeight(R : ANALYTIC_STRUCT_EXT).
       intros X Y ?. by econstructor.
   Qed.
 
-  Local Lemma bunch_equiv_fill_1 Δ C ϕ :
-    fill C (frml ϕ) =? Δ →
-    ∃ C', Δ = fill C' (frml ϕ) ∧ (∀ Δ, fill C' Δ ≡ fill C Δ).
+  Local Lemma bunch_equiv_fill_1 Δ Π ϕ :
+    fill Π (frml ϕ) =? Δ →
+    ∃ C', Δ = fill C' (frml ϕ) ∧ (∀ Δ, fill C' Δ ≡ fill Π Δ).
   Proof.
     intros Heq.
-    remember (fill C (frml ϕ)) as Y.
-    revert C HeqY.
+    remember (fill Π (frml ϕ)) as Y.
+    revert Π HeqY.
     induction Heq=>C' heqY; symmetry in heqY.
     + apply bunch_decomp_complete in heqY.
       apply bunch_decomp_ctx in heqY.
@@ -67,7 +64,7 @@ Module SeqcalcHeight(R : ANALYTIC_STRUCT_EXT).
       * destruct H1 as [C1 [HC0%bunch_decomp_correct HC]].
         destruct (IHHeq C1 HC0) as [C2 [HΔ1 HC2]].
         simplify_eq/=.
-        exists (C2 ++ C). rewrite fill_app. split; first done.
+        exists (C2 ++ Π). rewrite fill_app. split; first done.
         intros Δ. rewrite !fill_app HC2 //.
       * destruct H2 as (C1 & C2 & HC1 & HC2 & Hdec0).
         specialize (Hdec0 Δ2). apply bunch_decomp_correct in Hdec0.
@@ -160,13 +157,13 @@ Module SeqcalcHeight(R : ANALYTIC_STRUCT_EXT).
            by rewrite assoc.
   Qed.
 
-  Local Lemma bunch_equiv_fill_2 Δ C ϕ :
-    Δ =? fill C (frml ϕ) →
-    ∃ C', Δ = fill C' (frml ϕ) ∧ (∀ Δ, fill C' Δ ≡ fill C Δ).
+  Local Lemma bunch_equiv_fill_2 Δ Π ϕ :
+    Δ =? fill Π (frml ϕ) →
+    ∃ C', Δ = fill C' (frml ϕ) ∧ (∀ Δ, fill C' Δ ≡ fill Π Δ).
   Proof.
     intros Heq.
-    remember (fill C (frml ϕ)) as Y.
-    revert C HeqY.
+    remember (fill Π (frml ϕ)) as Y.
+    revert Π HeqY.
     induction Heq=>C' heqY; symmetry in heqY.
     + apply bunch_decomp_complete in heqY.
       apply bunch_decomp_ctx in heqY.
@@ -174,7 +171,7 @@ Module SeqcalcHeight(R : ANALYTIC_STRUCT_EXT).
       * destruct H1 as [C1 [HC0%bunch_decomp_correct HC]].
         destruct (IHHeq C1 HC0) as [C2 [HΔ1 HC2]].
         simplify_eq/=.
-        exists (C2 ++ C). rewrite fill_app. split; first done.
+        exists (C2 ++ Π). rewrite fill_app. split; first done.
         intros Δ. rewrite !fill_app HC2 //.
       * destruct H2 as (C1 & C2 & HC1 & HC2 & Hdec0).
         specialize (Hdec0 Δ1). apply bunch_decomp_correct in Hdec0.
@@ -222,7 +219,7 @@ Module SeqcalcHeight(R : ANALYTIC_STRUCT_EXT).
             by rewrite H4. }
            intros Δ. rewrite !fill_app/=.
            by rewrite assoc.
-    + exists (C' ++ [CtxSemicR ∅ₐ]%B). simpl; split.
+    + exists (C' ++ [ CtxSemicR ∅ₐ]%B). simpl; split.
       { rewrite fill_app /=. by rewrite heqY. }
       intros X; rewrite fill_app/=.
       by rewrite left_id.
@@ -263,13 +260,13 @@ Module SeqcalcHeight(R : ANALYTIC_STRUCT_EXT).
            by rewrite assoc.
   Qed.
 
-  Lemma bunch_equiv_fill Δ C ϕ :
-    Δ ≡ (fill C (frml ϕ)) →
-    ∃ C', Δ = fill C' (frml ϕ) ∧ (∀ Δ, fill C' Δ ≡ fill C Δ).
+  Lemma bunch_equiv_fill Δ Π ϕ :
+    Δ ≡ (fill Π (frml ϕ)) →
+    ∃ C', Δ = fill C' (frml ϕ) ∧ (∀ Δ, fill C' Δ ≡ fill Π Δ).
   Proof.
     intros H%bunch_equiv_2.
     revert Δ H. eapply rtc_ind_l.
-    { exists C. eauto. }
+    { exists Π. eauto. }
     intros X Y HXY HY. clear HY.
     intros (C0 & -> & HC0).
     destruct HXY as [HXY|HXY].
@@ -291,50 +288,55 @@ Module SeqcalcHeight(R : ANALYTIC_STRUCT_EXT).
   | BI_Equiv Δ Δ' ϕ n :
       (Δ ≡ Δ') → (Δ ⊢ᴮ{n} ϕ) →
       Δ' ⊢ᴮ{S n} ϕ
-  | BI_Weaken C Δ Δ' ϕ n : (fill C Δ ⊢ᴮ{n} ϕ) →
-                         fill C (Δ ;, Δ') ⊢ᴮ{S n} ϕ
-  | BI_Contr C Δ ϕ n : (fill C (Δ ;, Δ) ⊢ᴮ{n} ϕ) →
-                     fill C Δ ⊢ᴮ{S n} ϕ
-  | BI_Simple_Ext Π (Δs : nat → bunch) n
-    (Ts : list bterm) (T : bterm) ϕ :
-    (Ts, T) ∈ rules →
-    (∀ Ti, Ti ∈ Ts → fill Π (bterm_ctx_act Ti Δs) ⊢ᴮ{n} ϕ) →
-    fill Π (bterm_ctx_act T Δs) ⊢ᴮ{S n} ϕ
-  (* multiplicatives *)
+  | BI_Weaken Π Δ Δ' ϕ n : (fill Π Δ ⊢ᴮ{n} ϕ) →
+                         fill Π (Δ ;, Δ') ⊢ᴮ{S n} ϕ
+  | BI_Contr Π Δ ϕ n : (fill Π (Δ ;, Δ) ⊢ᴮ{n} ϕ) →
+                     fill Π Δ ⊢ᴮ{S n} ϕ
+  (* | BI_Cut Π Δ ϕ ψ : (Δ ⊢ᴮ ψ) → *)
+  (*                    (fill Π (frml ψ) ⊢ᴮ ϕ) → *)
+  (*                    fill Π Δ ⊢ᴮ ϕ *)
+  (* modal *)
+  | BI_Box_L Π ϕ ψ n :
+      (fill Π (frml ϕ) ⊢ᴮ{n} ψ) →
+      fill Π (frml (BOX ϕ)) ⊢ᴮ{S n} ψ
+  | BI_Box_R Δ ϕ n :
+      (BOX <$> Δ ⊢ᴮ{n} ϕ) →
+      BOX <$> Δ ⊢ᴮ{S n} BOX ϕ
+    (* multiplicatives *)
   | BI_Emp_R :
       ∅ₘ ⊢ᴮ{0} EMP
-  | BI_Emp_L C ϕ n :
-      (fill C ∅ₘ ⊢ᴮ{n} ϕ) →
-      fill C (frml EMP) ⊢ᴮ{S n} ϕ
+  | BI_Emp_L Π ϕ n :
+      (fill Π ∅ₘ ⊢ᴮ{n} ϕ) →
+      fill Π (frml EMP) ⊢ᴮ{S n} ϕ
   | BI_Sep_R Δ Δ' ϕ ψ n m :
       (Δ ⊢ᴮ{n} ϕ) →
       (Δ' ⊢ᴮ{m} ψ) →
       Δ ,, Δ' ⊢ᴮ{S (n `max` m)} SEP ϕ ψ
-  | BI_Sep_L C ϕ ψ χ n :
-      (fill C (frml ϕ ,, frml ψ) ⊢ᴮ{n} χ) →
-      fill C (frml (SEP ϕ ψ)) ⊢ᴮ{S n} χ
+  | BI_Sep_L Π ϕ ψ χ n :
+      (fill Π (frml ϕ ,, frml ψ) ⊢ᴮ{n} χ) →
+      fill Π (frml (SEP ϕ ψ)) ⊢ᴮ{S n} χ
   | BI_Wand_R Δ ϕ ψ n :
       (Δ ,, frml ϕ ⊢ᴮ{n} ψ) →
       Δ  ⊢ᴮ{S n} WAND ϕ ψ
-  | BI_Wand_L C Δ ϕ ψ χ n m :
+  | BI_Wand_L Π Δ ϕ ψ χ n m :
       (Δ ⊢ᴮ{n} ϕ) →
-      (fill C (frml ψ) ⊢ᴮ{m} χ) →
-      fill C (Δ ,, frml (WAND ϕ ψ)) ⊢ᴮ{S (n `max` m)} χ
+      (fill Π (frml ψ) ⊢ᴮ{m} χ) →
+      fill Π (Δ ,, frml (WAND ϕ ψ)) ⊢ᴮ{S (n `max` m)} χ
     (* additives *)
-  | BI_False_L C ϕ :
-      fill C (frml BOT) ⊢ᴮ{0} ϕ
+  | BI_False_L Π ϕ :
+      fill Π (frml BOT) ⊢ᴮ{0} ϕ
   | BI_True_R Δ :
       Δ ⊢ᴮ{0} TOP
-  | BI_True_L C ϕ n :
-      (fill C ∅ₐ ⊢ᴮ{n} ϕ) →
-      fill C (frml TOP) ⊢ᴮ{S n} ϕ
+  | BI_True_L Π ϕ n :
+      (fill Π ∅ₐ ⊢ᴮ{n} ϕ) →
+      fill Π (frml TOP) ⊢ᴮ{S n} ϕ
   | BI_Conj_R Δ Δ' ϕ ψ n m :
       (Δ ⊢ᴮ{n} ϕ) →
       (Δ' ⊢ᴮ{m} ψ) →
       Δ ;, Δ' ⊢ᴮ{S (n `max` m)} CONJ ϕ ψ
-  | BI_Conj_L C ϕ ψ χ n :
-      (fill C (frml ϕ ;, frml ψ) ⊢ᴮ{n} χ) →
-      fill C (frml (CONJ ϕ ψ)) ⊢ᴮ{S n} χ
+  | BI_Conj_L Π ϕ ψ χ n :
+      (fill Π (frml ϕ ;, frml ψ) ⊢ᴮ{n} χ) →
+      fill Π (frml (CONJ ϕ ψ)) ⊢ᴮ{S n} χ
   | BI_Disj_R1 Δ ϕ ψ n :
       (Δ ⊢ᴮ{n} ϕ) →
       Δ ⊢ᴮ{S n} DISJ ϕ ψ
@@ -348,24 +350,38 @@ Module SeqcalcHeight(R : ANALYTIC_STRUCT_EXT).
   | BI_Impl_R Δ ϕ ψ n :
       (Δ ;, frml ϕ ⊢ᴮ{n} ψ) →
       Δ  ⊢ᴮ{S n} IMPL ϕ ψ
-  | BI_Impl_L C Δ ϕ ψ χ n m:
+  | BI_Impl_L Π Δ ϕ ψ χ n m:
       (Δ ⊢ᴮ{n} ϕ) →
-      (fill C (frml ψ) ⊢ᴮ{m} χ) →
-      fill C (Δ ;, frml (IMPL ϕ ψ)) ⊢ᴮ{S (n `max` m)} χ
+      (fill Π (frml ψ) ⊢ᴮ{m} χ) →
+      fill Π (Δ ;, frml (IMPL ϕ ψ)) ⊢ᴮ{S (n `max` m)} χ
   where "Δ ⊢ᴮ{ n } ϕ" := (proves Δ%B ϕ%B n).
 
   Lemma provesN_proves n Δ ϕ :
     (Δ ⊢ᴮ{ n } ϕ) → Δ ⊢ᴮ ϕ.
   Proof.
-    induction 1; try by econstructor; eauto.
-    (* XXX: somehow, [try] is really needed here ^ *)
-  Qed.
-
-  Lemma proves_le n m Δ ϕ :
-    n ≤ m → (Δ ⊢ᴮ{n} ϕ) → Δ ⊢ᴮ{m} ϕ.
-  Proof.
-    induction 1; auto.
-    intros H1. eapply BI_Higher. eauto.
+    induction 1; eauto.
+    by econstructor; eauto.
+    by econstructor; eauto.
+    by econstructor; eauto.
+    by econstructor; eauto.
+    by econstructor; eauto.
+    by econstructor; eauto.
+    by econstructor; eauto.
+    by econstructor; eauto.
+    by econstructor; eauto.
+    by econstructor; eauto.
+    by econstructor; eauto.
+    by econstructor; eauto.
+    by econstructor; eauto.
+    by econstructor; eauto.
+    by econstructor; eauto.
+    by econstructor; eauto.
+    by econstructor; eauto.
+    by econstructor; eauto.
+    by econstructor; eauto.
+    by econstructor; eauto.
+    by econstructor; eauto.
+    by econstructor; eauto.
   Qed.
 
   Lemma proves_provesN Δ ϕ :
@@ -376,34 +392,18 @@ Module SeqcalcHeight(R : ANALYTIC_STRUCT_EXT).
     all: try (destruct IHproves1 as [n1 IH1];
               destruct IHproves2 as [n2 IH2]).
     all: try by eexists; econstructor; eauto.
-    (* The worst case: simple structural rules *)
-    apply (Forall_forall (λ Ti, ∃ n : nat, fill Π (bterm_ctx_act Ti Δs) ⊢ᴮ{ n} ϕ)) in H1.
-    apply Forall_exists_Forall2 in H1.
-    destruct H1 as (ns & Hns).
-    exists (S (max_list ns)).
-    eapply BI_Simple_Ext; eauto.
-    intros Ti HTi.
-    destruct (elem_of_list_lookup_1 _ _ HTi) as [i Hi].
-    destruct (ns !! i) as [n|] eqn:Hn; last first.
-    { eapply Forall2_lookup_r in Hns; eauto.
-      naive_solver. }
-    eapply (proves_le n). {
-      eapply max_list_elem_of_le.
-      by eapply elem_of_list_lookup_2.
-    }
-    eapply Forall2_lookup_lr in Hns; eauto.
   Qed.
 
   (** * Inversion lemmas *)
   Local Ltac bind_ctx :=
     match goal with
-    | [ |- fill ?C ?Δ,, ?Δ' ⊢ᴮ{_} _ ] =>
-      replace (fill C Δ,, Δ')%B
-      with (fill (C ++ [CtxCommaL Δ']) Δ)%B
+    | [ |- fill ?Π ?Δ,, ?Δ' ⊢ᴮ{_} _ ] =>
+      replace (fill Π Δ,, Δ')%B
+      with (fill (Π ++ [CtxCommaL Δ']) Δ)%B
       by rewrite fill_app//
-    | [ |- fill ?C ?Δ;, ?Δ' ⊢ᴮ{_} _ ] =>
-      replace (fill C Δ;, Δ')%B
-      with (fill (C ++ [CtxSemicL Δ']) Δ)%B
+    | [ |- fill ?Π ?Δ;, ?Δ' ⊢ᴮ{_} _ ] =>
+      replace (fill Π Δ;, Δ')%B
+      with (fill (Π ++ [CtxSemicL Δ']) Δ)%B
       by rewrite fill_app//
     end.
 
@@ -423,10 +423,6 @@ Module SeqcalcHeight(R : ANALYTIC_STRUCT_EXT).
     - intros ->. eapply BI_Equiv.
       { rewrite -H. reflexivity. }
       by apply IHproves.
-    - intros ->. bind_ctx.
-      eapply BI_Simple_Ext; eauto.
-      intros Ti HTi. rewrite fill_app. simpl.
-      eapply H1; eauto.
     - intros ?; simplify_eq/=. by apply BI_Higher.
     - commute_left_rule IHproves2.
     - intros ?; simplify_eq/=.
@@ -448,10 +444,6 @@ Module SeqcalcHeight(R : ANALYTIC_STRUCT_EXT).
     - intros ->. eapply BI_Equiv.
       { rewrite -H. reflexivity. }
       by apply IHproves.
-    - intros ->. bind_ctx.
-      eapply BI_Simple_Ext; eauto.
-      intros Ti HTi. rewrite fill_app. simpl.
-      eapply H1; eauto.
     - commute_left_rule IHproves2.
     - intros ?; simplify_eq/=.
       bind_ctx. eapply BI_Disj_L.
@@ -459,6 +451,249 @@ Module SeqcalcHeight(R : ANALYTIC_STRUCT_EXT).
       + rewrite fill_app/=. by eapply IHproves2.
     - intros ?; simplify_eq/=. by apply BI_Higher.
     - commute_left_rule IHproves2.
+  Qed.
+
+  Lemma box_l_inv' Δ Π ϕ χ n :
+    (Δ ⊢ᴮ{n} χ) →
+    Δ = fill Π (frml (BOX (BOX ϕ))) →
+    (fill Π (frml (BOX ϕ)) ⊢ᴮ{n} χ).
+  Proof.
+    revert Π Δ χ.
+    induction n using lt_wf_ind. rename H into IHproves.
+    intros Π Δ χ PROOF Heq. symmetry in Heq. revert Heq.
+    inversion PROOF; simplify_eq/= => Heq.
+    - (* raising the pf height *)
+      apply BI_Higher.
+      eapply IHproves; eauto.
+    - (* axiom *)
+      apply fill_is_frml in Heq. destruct_and!; simplify_eq/=.
+    - (* equivalence of bunches *)
+      simplify_eq/=.
+      destruct (bunch_equiv_fill _ _ _ H) as [Π2 [-> HΠ2]].
+      eapply BI_Equiv.
+      { apply HΠ2. }
+      eapply IHproves; eauto.
+    - (* weakening *)
+      apply bunch_decomp_complete in Heq.
+      apply bunch_decomp_ctx in Heq.
+      destruct Heq as [H1 | H2].
+      + destruct H1 as [Π1 [HΠ0 HΠ]].
+        inversion HΠ0; simplify_eq/=.
+        * rewrite !fill_app/=.
+          apply BI_Weaken.
+          rewrite -fill_app.
+          eapply IHproves; eauto.
+          by apply bunch_decomp_correct, bunch_decomp_app.
+        * rewrite !fill_app/=.
+          by apply BI_Weaken.
+      + rename Π into Π'.
+        rename Π0 into Π0'.
+        destruct H2 as (Π0 & Π1 & HΠ0 & HΠ1 & Hdec0).
+        rewrite -HΠ1.
+        apply BI_Weaken.
+        rewrite -HΠ0.
+        eapply IHproves; eauto.
+        apply bunch_decomp_correct. apply Hdec0.
+    - (* contraction *)
+      apply bunch_decomp_complete in Heq.
+      apply bunch_decomp_ctx in Heq.
+      destruct Heq as [H1 | H2]; last first.
+      + rename Π0 into Π0'.
+        destruct H2 as (Π0 & Π1 & HΠ0 & HΠ1 & Hdec0).
+        rewrite -HΠ1.
+        apply BI_Contr.
+        rewrite -HΠ0.
+        eapply IHproves; eauto.
+        apply bunch_decomp_correct. apply Hdec0.
+      + destruct H1 as [C0 [HC0 ->]].
+        apply bunch_decomp_correct in HC0.
+        simplify_eq/=.
+        rename Π0 into Π.
+        assert (fill Π (fill C0 (frml (BOX ϕ));, fill C0 (frml (BOX (BOX ϕ)))) ⊢ᴮ{ n0} χ) as IH1.
+        { specialize (IHproves n0 (lt_n_Sn _)).
+          set (C2 := (C0 ++ [CtxSemicL (fill C0 (frml (BOX (BOX ϕ))))] ++ Π)%B).
+          specialize (IHproves C2 _ _ H).
+          revert IHproves. rewrite /C2 !fill_app /=.
+          eauto. }
+        rewrite fill_app.
+        apply BI_Contr.
+        set (C2 := (C0 ++ [CtxSemicR (fill C0 (frml (BOX ϕ)))] ++ Π)%B).
+        replace (fill Π (fill C0 (frml (BOX ϕ));, fill C0 (frml (BOX ϕ))))%B
+                   with (fill C2 (frml (BOX ϕ)))%B by rewrite fill_app//.
+        eapply IHproves; eauto.
+        rewrite /C2 fill_app/=//.
+    - (* box L *)
+      apply bunch_decomp_complete in Heq.
+      apply bunch_decomp_ctx in Heq.
+      destruct Heq as [H1 | H2].
+      + destruct H1 as [C1 [HC0 HC]].
+        inversion HC0; simplify_eq/=.
+        by apply BI_Higher.
+      + destruct H2 as (C0 & C1 & HC0 & HC1 & Hdec0).
+        rewrite -HC1.
+        apply BI_Box_L.
+        rewrite -HC0.
+        eapply IHproves; eauto.
+        apply bunch_decomp_correct. apply Hdec0.
+    - (* box R *)
+      apply bunch_decomp_complete in Heq.
+      apply bunch_decomp_box in Heq.
+      destruct Heq as (Π' & -> & ->%bunch_decomp_correct).
+      change (frml (BOX ϕ)) with (BOX <$> (frml ϕ)).
+      rewrite -(bunch_map_fill BOX). apply BI_Box_R.
+      rewrite bunch_map_fill /=. eapply IHproves; eauto.
+      rewrite bunch_map_fill //.
+    - (* emp R *)
+      exfalso.
+      apply bunch_decomp_complete in Heq.
+      inversion Heq.
+    - (* emp L *)
+      apply bunch_decomp_complete in Heq.
+      apply bunch_decomp_ctx in Heq.
+      destruct Heq as [H1 | H2].
+      + destruct H1 as [C1 [HC0 HC]].
+        inversion HC0; simplify_eq/=.
+      + destruct H2 as (C0 & C1 & HC0 & HC1 & Hdec0).
+        rewrite -HC1.
+        apply BI_Emp_L.
+        rewrite -HC0.
+        eapply IHproves; eauto.
+        apply bunch_decomp_correct. apply Hdec0.
+    - (* sep R *)
+      apply bunch_decomp_complete in Heq.
+      inversion Heq; simplify_eq/=.
+      + rewrite fill_app /=.
+        eapply BI_Sep_R; eauto.
+        eapply IHproves; eauto; first lia.
+        by apply bunch_decomp_correct.
+      + rewrite fill_app /=.
+        eapply BI_Sep_R; eauto.
+        eapply IHproves; eauto; first lia.
+        by apply bunch_decomp_correct.
+    - (* sep L *)
+      apply bunch_decomp_complete in Heq.
+      apply bunch_decomp_ctx in Heq.
+      destruct Heq as [H1 | H2].
+      + destruct H1 as [C1 [HC0 HC]].
+        inversion HC0; simplify_eq/=.
+      + destruct H2 as (C0 & C1 & HC0 & HC1 & Hdec0).
+        rewrite -HC1.
+        apply BI_Sep_L.
+        rewrite -HC0.
+        eapply IHproves; eauto.
+        apply bunch_decomp_correct. apply Hdec0.
+    - (* wand R *)
+      apply BI_Wand_R.
+      assert ((fill Π (frml (BOX ϕ)),, frml ϕ0) =
+                   fill (Π ++ [CtxCommaL (frml ϕ0)]) (frml (BOX ϕ)))%B as ->.
+      { rewrite fill_app//. }
+      eapply IHproves; eauto. rewrite -Heq fill_app /= //.
+    - (* wand L *)
+      apply bunch_decomp_complete in Heq.
+      apply bunch_decomp_ctx in Heq.
+      destruct Heq as [H1 | H2].
+      + destruct H1 as [C1 [HC0 HC]].
+        inversion HC0; simplify_eq/=.
+        * rewrite !fill_app/=.
+          eapply BI_Wand_L; eauto.
+          eapply IHproves; eauto; first lia.
+          by apply bunch_decomp_correct.
+        * exfalso. inversion H6.
+      + destruct H2 as (C0 & C1 & HC0 & HC1 & Hdec0).
+        rewrite -HC1.
+        apply BI_Wand_L; eauto.
+        rewrite -HC0.
+        eapply IHproves; eauto; first lia.
+        apply bunch_decomp_correct. apply Hdec0.
+    - (* bot L *)
+      apply bunch_decomp_complete in Heq.
+      apply bunch_decomp_ctx in Heq.
+      destruct Heq as [H1 | H2].
+      + destruct H1 as [C1 [HC0 HC]].
+        inversion HC0; simplify_eq/=.
+      + destruct H2 as (C0 & C1 & HC0 & HC1 & Hdec0).
+        rewrite -HC1.
+        apply BI_False_L.
+    - (* top R *) apply BI_True_R.
+    - (* top L *)
+      apply bunch_decomp_complete in Heq.
+      apply bunch_decomp_ctx in Heq.
+      destruct Heq as [H1 | H2].
+      + destruct H1 as [C1 [HC0 HC]].
+        inversion HC0; simplify_eq/=.
+      + destruct H2 as (C0 & C1 & HC0 & HC1 & Hdec0).
+        rewrite -HC1.
+        apply BI_True_L.
+        rewrite -HC0.
+        eapply IHproves; eauto.
+        apply bunch_decomp_correct. apply Hdec0.
+    - (* conjR *)
+      apply bunch_decomp_complete in Heq.
+      inversion Heq; simplify_eq/=.
+      + rewrite fill_app /=.
+        eapply BI_Conj_R; eauto.
+        eapply IHproves; eauto; first lia.
+        by apply bunch_decomp_correct.
+      + rewrite fill_app /=.
+        eapply BI_Conj_R; eauto.
+        eapply IHproves; eauto; first lia.
+        by apply bunch_decomp_correct.
+    - (* conjL *)
+      apply bunch_decomp_complete in Heq.
+      apply bunch_decomp_ctx in Heq.
+      destruct Heq as [H1 | H2].
+      + destruct H1 as [C1 [HC0 HC]].
+        inversion HC0; simplify_eq/=.
+      + destruct H2 as (C0 & C1 & HC0 & HC1 & Hdec0).
+        rewrite -HC1.
+        apply BI_Conj_L.
+        rewrite -HC0.
+        eapply IHproves; eauto.
+        apply bunch_decomp_correct. apply Hdec0.
+    - (* disj R 1 *)
+      eapply BI_Disj_R1.
+      eapply IHproves; eauto.
+    - (* disj R 2 *)
+      eapply BI_Disj_R2.
+      eapply IHproves; eauto.
+    - (* disj L *)
+      apply bunch_decomp_complete in Heq.
+      apply bunch_decomp_ctx in Heq.
+      destruct Heq as [H1 | H2].
+      + destruct H1 as [C1 [HC0 HC]].
+        inversion HC0; simplify_eq/=.
+      + destruct H2 as (C0 & C1 & HC0 & HC1 & Hdec0).
+        rewrite -HC1.
+        apply BI_Disj_L.
+        * rewrite -HC0.
+          eapply IHproves; eauto; first lia.
+          apply bunch_decomp_correct. apply Hdec0.
+        * rewrite -HC0.
+          eapply IHproves; eauto; first lia.
+          apply bunch_decomp_correct. apply Hdec0.
+    - (* impl R *)
+      apply BI_Impl_R.
+      assert ((fill Π (frml (BOX ϕ));, frml ϕ0) =
+                   fill (Π ++ [CtxSemicL (frml ϕ0)]) (frml (BOX ϕ)))%B as ->.
+      { rewrite fill_app//. }
+      eapply IHproves; eauto. rewrite -Heq fill_app /= //.
+    - (* impl L *)
+      apply bunch_decomp_complete in Heq.
+      apply bunch_decomp_ctx in Heq.
+      destruct Heq as [H1 | H2].
+      + destruct H1 as [C1 [HC0 HC]].
+        inversion HC0; simplify_eq/=.
+        * rewrite !fill_app/=.
+          eapply BI_Impl_L; eauto.
+          eapply IHproves; eauto; first lia.
+          by apply bunch_decomp_correct.
+        * exfalso. inversion H6.
+      + destruct H2 as (C0 & C1 & HC0 & HC1 & Hdec0).
+        rewrite -HC1.
+        apply BI_Impl_L; eauto.
+        rewrite -HC0.
+        eapply IHproves; eauto; first lia.
+        apply bunch_decomp_correct. apply Hdec0.
   Qed.
 
   Lemma collapse_l_inv' Δ Π Δ' ϕ χ n :
@@ -497,8 +732,7 @@ Module SeqcalcHeight(R : ANALYTIC_STRUCT_EXT).
           by apply bunch_decomp_correct, bunch_decomp_app.
         * rewrite !fill_app/=.
           by apply BI_Weaken.
-      + rename C into C'.
-        destruct H2 as (C0 & C1 & HC0 & HC1 & Hdec0).
+      + destruct H2 as (C0 & C1 & HC0 & HC1 & Hdec0).
         rewrite -HC1.
         apply BI_Weaken.
         rewrite -HC0.
@@ -508,77 +742,48 @@ Module SeqcalcHeight(R : ANALYTIC_STRUCT_EXT).
       apply bunch_decomp_complete in Heq.
       apply bunch_decomp_ctx in Heq.
       destruct Heq as [H1 | H2]; last first.
-      + rename C into C'.
-        destruct H2 as (C0 & C1 & HC0 & HC1 & Hdec0).
-        rewrite -HC1.
-        apply BI_Contr.
-        rewrite -HC0.
-        eapply IHproves; eauto.
-        apply bunch_decomp_correct. apply Hdec0.
-      + rename C into C'.
-        destruct H1 as [C0 [HC0 ->]].
-        apply bunch_decomp_correct in HC0.
-        simplify_eq/=.
-        assert (fill C' (fill C0 Δ';, fill C0 (frml ϕ)) ⊢ᴮ{ n0} χ) as IH1.
-        { specialize (IHproves n0 (lt_n_Sn _)).
-          set (C2 := (C0 ++ [CtxSemicL (fill C0 (frml ϕ))] ++ C')%B).
-          specialize (IHproves C2 _ _ _ _ Hcoll H).
-          revert IHproves. rewrite /C2 !fill_app /=.
-          eauto. }
-        rewrite fill_app.
-        apply BI_Contr.
-        set (C2 := (C0 ++ [CtxSemicR (fill C0 Δ')] ++ C')%B).
-        replace (fill C' (fill C0 Δ';, fill C0 Δ'))%B
-                   with (fill C2 Δ')%B by rewrite fill_app//.
-        eapply IHproves; eauto.
-        rewrite /C2 fill_app//.
-    - (* ext *)
-      apply bunch_decomp_complete in Heq.
-      apply bunch_decomp_ctx in Heq.
-      destruct Heq as [H1 | H2]; last first.
       + destruct H2 as (C0 & C1 & HC0 & HC1 & Hdec0).
         rewrite -HC1.
-        eapply BI_Simple_Ext; eauto.
-        intros Ti Hi.
+        apply BI_Contr.
         rewrite -HC0.
         eapply IHproves; eauto.
         apply bunch_decomp_correct. apply Hdec0.
       + destruct H1 as [C0 [HC0 ->]].
         apply bunch_decomp_correct in HC0.
         simplify_eq/=.
-        apply bterm_ctx_act_decomp in HC0; last first.
-        { by eapply (rules_good (Ts,T)). }
-        destruct HC0 as (j & Π₀ & Hjfv & Hj & HC0).
-        rewrite fill_app -HC0.
-        eapply BI_Simple_Ext; eauto.
-        revert Hj Hjfv IHproves H0 Hcoll.
-        clear.
-        intros Hj Hjfv IHproves Hpfs Hcoll.
-        intros Ti HTi. specialize (Hpfs Ti HTi).
-        revert Π0 Hpfs. clear HTi.
-        induction Ti=>Π0 Hpfs.
-        { simpl.
-          destruct (decide (j = x)) as [->|?].
-          - rewrite functions.fn_lookup_insert.
-            rewrite -fill_app. simpl in Hpfs.
-            eapply IHproves; eauto.
-            by rewrite fill_app -Hj.
-          - rewrite functions.fn_lookup_insert_ne; auto. }
-        { simpl.
-          assert (fill ([CtxL sp (bterm_ctx_act Ti2 Δs)]++Π0) (bterm_ctx_act Ti1 (<[j:=fill Π₀ Δ']> Δs)) ⊢ᴮ{ n0} χ) as HH1.
-          { eapply IHTi1. rewrite fill_app /=. eauto. }
-          rewrite fill_app in HH1.
-          simpl in HH1.
-          replace
-            (fill Π0 (bbin sp
-                       (bterm_ctx_act Ti1
-             (<[j:=fill Π₀ Δ']> Δs)) (bterm_ctx_act Ti2 (<[j:=fill Π₀ Δ']> Δs))))%B
-            with
-          (fill ([CtxR sp (bterm_ctx_act Ti1 (<[j:=fill Π₀ Δ']> Δs))]++Π0)
-                (bterm_ctx_act Ti2 (<[j:=fill Π₀ Δ']> Δs)))%B
-            by rewrite fill_app//.
-          eapply IHTi2.
-          rewrite fill_app/=//. }
+        assert (fill Π0 (fill C0 Δ';, fill C0 (frml ϕ)) ⊢ᴮ{ n0} χ) as IH1.
+        { specialize (IHproves n0 (lt_n_Sn _)).
+          set (C2 := (C0 ++ [CtxSemicL (fill C0 (frml ϕ))] ++ Π0)%B).
+          specialize (IHproves C2 _ _ _ _ Hcoll H).
+          revert IHproves. rewrite /C2 !fill_app /=.
+          eauto. }
+        rewrite fill_app.
+        apply BI_Contr.
+        set (C2 := (C0 ++ [CtxSemicR (fill C0 Δ')] ++ Π0)%B).
+        replace (fill Π0 (fill C0 Δ';, fill C0 Δ'))%B
+                   with (fill C2 Δ')%B by rewrite fill_app//.
+        eapply IHproves; eauto.
+        rewrite /C2 fill_app//.
+    - (* box L *)
+      apply bunch_decomp_complete in Heq.
+      apply bunch_decomp_ctx in Heq.
+      destruct Heq as [H1 | H2].
+      + destruct H1 as [C1 [HC0 HC]].
+        inversion HC0; simplify_eq/=.
+        inversion Hcoll; simplify_eq/=.
+        apply BI_Box_L; done.
+      + destruct H2 as (C0 & C1 & HC0 & HC1 & Hdec0).
+        rewrite -HC1.
+        apply BI_Box_L.
+        rewrite -HC0.
+        eapply IHproves; eauto.
+        apply bunch_decomp_correct. apply Hdec0.
+    - (* box R *)
+      assert (∃ ψ, ϕ = BOX ψ) as [ψ Hψ].
+      { eapply bunch_decomp_box_frml.
+        by apply bunch_decomp_complete. }
+      subst. inversion Hcoll; simplify_eq/=.
+      rewrite Heq. by apply BI_Box_R.
     - (* emp R *)
       exfalso.
       apply bunch_decomp_complete in Heq.
@@ -592,8 +797,7 @@ Module SeqcalcHeight(R : ANALYTIC_STRUCT_EXT).
         inversion Hcoll; simplify_eq/=.
         * by apply BI_Emp_L.
         * by apply BI_Higher.
-      + rename C into C'.
-        destruct H2 as (C0 & C1 & HC0 & HC1 & Hdec0).
+      + destruct H2 as (C0 & C1 & HC0 & HC1 & Hdec0).
         rewrite -HC1.
         apply BI_Emp_L.
         rewrite -HC0.
@@ -617,18 +821,17 @@ Module SeqcalcHeight(R : ANALYTIC_STRUCT_EXT).
       + destruct H1 as [C1 [HC0 HC]].
         inversion HC0; simplify_eq/=.
         inversion Hcoll; simplify_eq/=; eauto.
-        assert (fill C (Δ1,, frml ψ) ⊢ᴮ{ n0} χ) as H1.
-        { replace (fill C (Δ1,, frml ψ))%B
-            with (fill ([CtxCommaL (frml ψ)]++C) Δ1)
+        assert (fill Π0 (Δ1,, frml ψ) ⊢ᴮ{ n0} χ) as H1.
+        { replace (fill Π0 (Δ1,, frml ψ))%B
+            with (fill ([CtxCommaL (frml ψ)]++Π0) Δ1)
             by rewrite fill_app//.
           eapply IHproves; eauto. }
-        replace (fill C (Δ1,, Δ2))%B
-          with (fill ([CtxCommaR Δ1]++C) Δ2)
+        replace (fill Π0 (Δ1,, Δ2))%B
+          with (fill ([CtxCommaR Δ1]++Π0) Δ2)
           by rewrite fill_app//.
         apply BI_Higher.
         eapply IHproves; eauto.
-      + rename C into C'.
-        destruct H2 as (C0 & C1 & HC0 & HC1 & Hdec0).
+      + destruct H2 as (C0 & C1 & HC0 & HC1 & Hdec0).
         rewrite -HC1.
         apply BI_Sep_L.
         rewrite -HC0.
@@ -654,8 +857,7 @@ Module SeqcalcHeight(R : ANALYTIC_STRUCT_EXT).
           inversion Hcoll; subst.
           simpl.
           eapply BI_Wand_L; eauto.
-      + rename C into C'.
-        destruct H2 as (C0 & C1 & HC0 & HC1 & Hdec0).
+      + destruct H2 as (C0 & C1 & HC0 & HC1 & Hdec0).
         rewrite -HC1.
         apply BI_Wand_L; eauto.
         rewrite -HC0.
@@ -668,8 +870,7 @@ Module SeqcalcHeight(R : ANALYTIC_STRUCT_EXT).
       + destruct H1 as [C1 [HC0 HC]].
         inversion HC0; simplify_eq/=.
         inversion Hcoll; eauto.
-      + rename C into C'.
-        destruct H2 as (C0 & C1 & HC0 & HC1 & Hdec0).
+      + destruct H2 as (C0 & C1 & HC0 & HC1 & Hdec0).
         rewrite -HC1.
         apply BI_False_L.
     - (* top R *) apply BI_True_R.
@@ -681,8 +882,7 @@ Module SeqcalcHeight(R : ANALYTIC_STRUCT_EXT).
         inversion HC0; simplify_eq/=.
         inversion Hcoll; subst; eauto.
         by apply BI_Higher.
-      + rename C into C'.
-        destruct H2 as (C0 & C1 & HC0 & HC1 & Hdec0).
+      + destruct H2 as (C0 & C1 & HC0 & HC1 & Hdec0).
         rewrite -HC1.
         apply BI_True_L.
         rewrite -HC0.
@@ -706,18 +906,17 @@ Module SeqcalcHeight(R : ANALYTIC_STRUCT_EXT).
       + destruct H1 as [C1 [HC0 HC]].
         inversion HC0; simplify_eq/=.
         inversion Hcoll; simplify_eq/=; eauto.
-        assert (fill C (Δ1;, frml ψ) ⊢ᴮ{ n0} χ) as H1.
-        { replace (fill C (Δ1;, frml ψ))%B
-            with (fill ([CtxSemicL (frml ψ)]++C) Δ1)
+        assert (fill Π0 (Δ1;, frml ψ) ⊢ᴮ{ n0} χ) as H1.
+        { replace (fill Π0 (Δ1;, frml ψ))%B
+            with (fill ([CtxSemicL (frml ψ)]++Π0) Δ1)
             by rewrite fill_app//.
           eapply IHproves; eauto. }
-        replace (fill C (Δ1;, Δ2))%B
-          with (fill ([CtxSemicR Δ1]++C) Δ2)
+        replace (fill Π0 (Δ1;, Δ2))%B
+          with (fill ([CtxSemicR Δ1]++Π0) Δ2)
           by rewrite fill_app//.
         apply BI_Higher.
         eapply IHproves; eauto.
-      + rename C into C'.
-        destruct H2 as (C0 & C1 & HC0 & HC1 & Hdec0).
+      + destruct H2 as (C0 & C1 & HC0 & HC1 & Hdec0).
         rewrite -HC1.
         apply BI_Conj_L.
         rewrite -HC0.
@@ -762,8 +961,7 @@ Module SeqcalcHeight(R : ANALYTIC_STRUCT_EXT).
           by apply bunch_decomp_correct.
         * inversion H6; subst.
           inversion Hcoll; simplify_eq/=; eauto.
-      + rename C into C'.
-        destruct H2 as (C0 & C1 & HC0 & HC1 & Hdec0).
+      + destruct H2 as (C0 & C1 & HC0 & HC1 & Hdec0).
         rewrite -HC1.
         apply BI_Impl_L; eauto.
         rewrite -HC0.
@@ -771,48 +969,69 @@ Module SeqcalcHeight(R : ANALYTIC_STRUCT_EXT).
         apply bunch_decomp_correct. apply Hdec0.
   Qed.
 
-  (** Derivable rules / inversion lemmas *)
-  Lemma impl_r_inv Δ ϕ ψ :
-    (Δ ⊢ᴮ IMPL ϕ ψ) →
-    (Δ ;, frml ϕ ⊢ᴮ ψ)%B.
-  Proof.
-    intros [n H]%proves_provesN.
+
+(** Derivable rules / inversion lemmas *)
+
+Lemma impl_r_inv Δ ϕ ψ :
+  (Δ ⊢ᴮ IMPL ϕ ψ) →
+  (Δ ;, frml ϕ ⊢ᴮ ψ)%B.
+Proof.
+  intros [n H]%proves_provesN.
+  eapply provesN_proves.
+  by apply impl_r_inv'.
+Qed.
+Lemma wand_r_inv Δ ϕ ψ :
+  (Δ ⊢ᴮ WAND ϕ ψ) →
+  (Δ ,, frml ϕ ⊢ᴮ ψ)%B.
+Proof.
+  intros [n H]%proves_provesN.
+  eapply provesN_proves.
+  by apply wand_r_inv'.
+Qed.
+Lemma sep_l_inv Π ϕ ψ χ :
+  (fill Π (frml (SEP ϕ ψ)) ⊢ᴮ χ) →
+  (fill Π (frml ϕ,, frml ψ) ⊢ᴮ χ).
+Proof.
+  intros [n H]%proves_provesN.
+  eapply provesN_proves.
+  eapply collapse_l_inv'; eauto.
+  by repeat constructor.
+Qed.
+Lemma conj_l_inv Π ϕ ψ χ :
+  (fill Π (frml (CONJ ϕ ψ)) ⊢ᴮ χ) →
+  (fill Π (frml ϕ;, frml ψ) ⊢ᴮ χ).
+Proof.
+  intros [n H]%proves_provesN.
+  eapply provesN_proves.
+  eapply collapse_l_inv'; eauto.
+  by repeat constructor.
+Qed.
+
+Lemma box_l_inv Π Δ ϕ :
+  (fill Π (BOX <$> (BOX <$> Δ)) ⊢ᴮ ϕ) →
+  (fill Π (BOX <$> Δ) ⊢ᴮ ϕ).
+Proof.
+  revert Π. induction Δ; simpl; eauto.
+  - intros Π [n H]%proves_provesN.
     eapply provesN_proves.
-    by apply impl_r_inv'.
-  Qed.
-  Lemma wand_r_inv Δ ϕ ψ :
-    (Δ ⊢ᴮ WAND ϕ ψ) →
-    (Δ ,, frml ϕ ⊢ᴮ ψ)%B.
-  Proof.
-    intros [n H]%proves_provesN.
-    eapply provesN_proves.
-    by apply wand_r_inv'.
-  Qed.
-  Lemma sep_l_inv C ϕ ψ χ :
-    (fill C (frml (SEP ϕ ψ)) ⊢ᴮ χ) →
-    (fill C (frml ϕ,, frml ψ) ⊢ᴮ χ).
-  Proof.
-    intros [n H]%proves_provesN.
-    eapply provesN_proves.
-    eapply collapse_l_inv'; eauto.
-    by repeat constructor.
-  Qed.
-  Lemma conj_l_inv C ϕ ψ χ :
-    (fill C (frml (CONJ ϕ ψ)) ⊢ᴮ χ) →
-    (fill C (frml ϕ;, frml ψ) ⊢ᴮ χ).
-  Proof.
-    intros [n H]%proves_provesN.
-    eapply provesN_proves.
-    eapply collapse_l_inv'; eauto.
-    by repeat constructor.
-  Qed.
-  Lemma BI_Collapse_L_inv C Δ ϕ :
-    (fill C (frml (collapse Δ)) ⊢ᴮ ϕ) →
-    (fill C Δ ⊢ᴮ ϕ).
-  Proof.
-    intros [n H]%proves_provesN.
-    eapply provesN_proves.
-    eapply collapse_l_inv'; eauto.
-    apply collapse_gr_sound.
-  Qed.
+    eapply box_l_inv'; eauto.
+  - intros Π H1.
+    change (fill Π (bbin s (BOX <$> Δ1) (BOX <$> Δ2)))%B
+      with (fill (CtxR s (BOX <$> Δ1)::Π) (BOX <$> Δ2)).
+    apply IHΔ2. simpl.
+    change (fill Π (bbin s (BOX <$> Δ1) (BOX <$> (BOX <$> Δ2))))%B
+      with (fill (CtxL s (BOX <$> (BOX <$> Δ2))::Π) (BOX <$> Δ1)).
+    apply IHΔ1. simpl. done.
+Qed.
+
+Lemma BI_Collapse_L_inv Π Δ ϕ :
+  (fill Π (frml (collapse Δ)) ⊢ᴮ ϕ) →
+  (fill Π Δ ⊢ᴮ ϕ).
+Proof.
+  intros [n H]%proves_provesN.
+  eapply provesN_proves.
+  eapply collapse_l_inv'; eauto.
+  apply collapse_gr_sound.
+Qed.
+
 End SeqcalcHeight.
