theories/bunches.v
@@ -1,0 +1,266 @@
+(* Bunches *)
+From Coq Require Import ssreflect.
+From stdpp Require Import prelude gmap fin_sets.
+From bunched.algebra Require Import bi.
+
+Declare Scope bunch_scope.
+Delimit Scope bunch_scope with B.
+
+(** * Generic syntax for bunches *)
+Inductive sep := Comma | SemiC.
+
+Inductive bunch {formula : Type} : Type :=
+| frml (ϕ : formula)
+| bnul (s : sep)
+| bbin (s : sep) (Δ Γ : bunch)
+.
+
+(* Definition semic {frml} (Δ Γ : @bunch frml) := bbin SemiC Δ Γ. *)
+(* Definition comma {frml} (Δ Γ : @bunch frml) := bbin Comma Δ Γ. *)
+(* Definition top {frml} : @bunch frml := bnul SemiC. *)
+(* Definition empty {frml} : @bunch frml := bnul Comma. *)
+
+Notation "∅ₐ" := (bnul SemiC) : bunch_scope.
+Notation "∅ₘ" := (bnul Comma) : bunch_scope.
+Notation "Δ ';,' Γ" := (bbin SemiC Δ%B Γ%B) (at level 80, right associativity) : bunch_scope.
+Notation "Δ ',,' Γ" := (bbin Comma Δ%B Γ%B) (at level 80, right associativity) : bunch_scope.
+
+(** ** Bunched contexts with a hole *)
+Inductive bunch_ctx_item {frml : Type} : Type :=
+| CtxL (s : sep) (Δ2 : @bunch frml)
+| CtxR (s : sep) (Δ1 : @bunch frml)
+.
+
+Definition CtxCommaL {frml} (Δ2 : bunch) : @bunch_ctx_item frml
+  := CtxL Comma Δ2.
+Definition CtxSemicL {frml} (Δ2 : bunch) : @bunch_ctx_item frml
+  := CtxL SemiC Δ2.
+Definition CtxCommaR {frml} (Δ1 : bunch) : @bunch_ctx_item frml
+  := CtxR Comma Δ1.
+Definition CtxSemicR {frml} (Δ1 : bunch) : @bunch_ctx_item frml
+  := CtxR SemiC Δ1.
+
+Definition bunch_ctx {frml} := list (@bunch_ctx_item frml).
+
+Definition fill_item {frml} (F : @bunch_ctx_item frml) (Δ : bunch) : bunch :=
+  match F with
+  | CtxL s Δ2 => bbin s Δ Δ2
+  | CtxR s Δ1 => bbin s Δ1 Δ
+  end.
+
+Definition fill {frml} (Π : @bunch_ctx frml) (Δ : bunch) : bunch :=
+  foldl (flip fill_item) Δ Π.
+
+#[global] Instance bunch_fmap : FMap (@bunch) :=
+  fix go A B f Δ {struct Δ} := let _ : FMap (@bunch) := @go in
+  match Δ with
+  | bnul s => bnul s
+  | bbin s Δ Δ' => bbin s (fmap f Δ) (fmap f Δ')
+  | frml ϕ => frml (f ϕ)
+  end%B.
+
+Definition bunch_ctx_item_map {A B} (f : A → B) (F : @bunch_ctx_item A) :=
+  match F with
+  | CtxL s Δ => CtxL s (f <$> Δ)
+  | CtxR s Δ => CtxR s (f <$> Δ)
+  end.
+
+Definition bunch_ctx_map {A B} (f : A → B) (Π : @bunch_ctx A) := map (bunch_ctx_item_map f) Π.
+
+
+(** ** Bunch equivalence *)
+(** Equivalence on bunches is defined to be the least congruence
+      that satisfies the monoidal laws for (empty and comma) and (top
+      and semicolon). *)
+Inductive bunch_equiv {frml} : @bunch frml → @bunch frml → Prop :=
+| BE_refl Δ : Δ =? Δ
+| BE_sym Δ1 Δ2 : Δ1 =? Δ2 → Δ2 =? Δ1
+| BE_trans Δ1 Δ2 Δ3 : Δ1 =? Δ2 → Δ2 =? Δ3 → Δ1 =? Δ3
+| BE_cong C Δ1 Δ2 : Δ1 =? Δ2 → fill C Δ1 =? fill C Δ2
+| BE_unit_l s Δ : bbin s (bnul s) Δ =? Δ
+| BE_comm s Δ1 Δ2 : bbin s Δ1 Δ2 =? bbin s Δ2 Δ1
+| BE_assoc s Δ1 Δ2 Δ3 : bbin s Δ1 (bbin s Δ2 Δ3) =? bbin s (bbin s Δ1 Δ2) Δ3
+where "Δ =? Γ" := (bunch_equiv Δ%B Γ%B).
+
+(** Register [bunch_equiv] as [(≡)] *)
+#[export] Instance equiv_bunch_equiv frml : Equiv (@bunch frml) := bunch_equiv.
+
+(** * Properties *)
+
+#[export] Instance equivalence_bunch_equiv frml : Equivalence ((≡@{@bunch frml})).
+Proof.
+  repeat split.
+  - intro x. econstructor.
+  - intros x y Hxy. by econstructor.
+  - intros x y z Hxy Hyz. by econstructor.
+Qed.
+
+#[export] Instance bbin_comm frml s : Comm (≡@{@bunch frml}) (bbin s).
+Proof. intros X Y. apply BE_comm. Qed.
+#[export] Instance bbin_assoc frml s : Assoc (≡@{@bunch frml}) (bbin s).
+Proof. intros X Y Z. apply BE_assoc. Qed.
+#[export] Instance bbin_leftid frml s : LeftId (≡@{@bunch frml}) (bnul s) (bbin s).
+Proof. intros X. apply BE_unit_l. Qed.
+#[export] Instance bbin_rightid frml s : RightId (≡@{@bunch frml}) (bnul s) (bbin s).
+Proof. intros X. rewrite comm. apply BE_unit_l. Qed.
+
+#[export] Instance fill_proper frml Π : Proper ((≡) ==> (≡@{@bunch frml})) (fill Π).
+Proof. intros X Y. apply BE_cong. Qed.
+
+#[export] Instance bbin_proper frml s : Proper ((≡) ==> (≡) ==> (≡@{@bunch frml})) (bbin s).
+Proof.
+  intros Δ1 Δ2 H Δ1' Δ2' H'.
+  change ((fill [CtxL s Δ1'] Δ1) ≡ (fill [CtxL s Δ2'] Δ2)).
+  etrans.
+  { eapply BE_cong; eauto. }
+  simpl.
+  change ((fill [CtxR s Δ2] Δ1') ≡ (fill [CtxR s Δ2] Δ2')).
+  eapply BE_cong; eauto.
+Qed.
+
+Lemma fill_app {frml} (Π Π' : @bunch_ctx frml) (Δ : bunch) :
+  fill (Π ++ Π') Δ = fill Π' (fill Π Δ).
+Proof. by rewrite /fill foldl_app. Qed.
+
+Lemma bunch_map_fill {A B} (f : A → B) Π Δ :
+  f <$> (fill Π Δ) = fill (bunch_ctx_map f Π) (f <$> Δ).
+Proof.
+  revert Δ. induction Π as [|F Π IH] =>Δ/=//.
+  rewrite IH. f_equiv. by destruct F; simpl.
+Qed.
+
+Global Instance bunch_map_proper {A B} (f : A → B) : Proper ((≡) ==> (≡@{bunch})) (fmap f).
+Proof.
+  intros Δ1 Δ2 HD. induction HD; simpl; eauto.
+  - etrans; eauto.
+  - rewrite !bunch_map_fill. by f_equiv.
+  - by rewrite left_id.
+  - by rewrite comm.
+  - by rewrite assoc.
+Qed.
+
+Section interp.
+  Variable (PROP : bi).
+  Context {formula : Type}.
+  Notation bunch := (@bunch formula).
+  Notation bunch_ctx := (@bunch_ctx formula).
+
+  Implicit Types (A B C : PROP).
+  Implicit Type Δ : bunch.
+  Implicit Type Π : bunch_ctx.
+
+  Variable (i : formula → PROP).
+
+  Definition sep_interp (sp : sep) : PROP → PROP → PROP :=
+    match sp with
+    | Comma => (∗)
+    | SemiC => (∧)
+    end%I.
+  #[export] Instance sep_interp_proper sp : Proper ((≡) ==> (≡) ==> (≡)) (sep_interp sp).
+  Proof. destruct sp; apply _. Qed.
+  #[export] Instance sep_interp_mono sp : Proper ((⊢) ==> (⊢) ==> (⊢)) (sep_interp sp).
+  Proof. destruct sp; apply _. Qed.
+
+  Fixpoint bunch_interp (Δ : bunch) : PROP :=
+    match Δ with
+    | frml ϕ => i ϕ
+    | ∅ₐ => True
+    | ∅ₘ => emp
+    | bbin sp Δ Δ' => sep_interp sp (bunch_interp Δ) (bunch_interp Δ')
+    end%B%I.
+
+    Definition bunch_ctx_item_interp (F : bunch_ctx_item) : PROP → PROP :=
+    λ P, match F with
+        | CtxL sp Δ => sep_interp sp P (bunch_interp Δ)
+        | CtxR sp Δ => sep_interp sp (bunch_interp Δ) P
+        end%I.
+
+  Definition bunch_ctx_interp Π : PROP → PROP :=
+    λ P, foldl (flip bunch_ctx_item_interp) P Π.
+
+  Lemma bunch_ctx_interp_cons F Π A :
+    bunch_ctx_interp (F::Π) A = bunch_ctx_interp Π (bunch_ctx_item_interp F A).
+  Proof. reflexivity. Qed.
+
+  Global Instance bunch_ctx_interp_proper Π : Proper ((≡) ==> (≡)) (bunch_ctx_interp Π).
+  Proof.
+    induction Π as [|F Π]=>X Y HXY.
+    - simpl; auto.
+    - simpl.
+      eapply IHΠ.
+      destruct F; solve_proper.
+  Qed.
+
+  Lemma bunch_ctx_interp_decomp Π Δ :
+    bunch_interp (fill Π Δ) ≡ bunch_ctx_interp Π (bunch_interp Δ).
+  Proof.
+    revert Δ. induction Π as [|C Π IH]=>Δ; first by reflexivity.
+    apply bi.equiv_entails_2.
+    - destruct C; simpl; by rewrite IH.
+    - destruct C; simpl; by rewrite IH.
+  Qed.
+
+  Lemma bunch_interp_fill_item_mono (C : bunch_ctx_item) Δ Δ' :
+    (bunch_interp Δ ⊢ bunch_interp Δ') →
+    bunch_interp (fill_item C Δ) ⊢ bunch_interp (fill_item C Δ').
+  Proof.
+    intros H1.
+    induction C as [ sp ? | sp ? ]; simpl; by rewrite H1.
+  Qed.
+
+  Lemma bunch_interp_fill_mono Π Δ Δ' :
+    (bunch_interp Δ ⊢ bunch_interp Δ') →
+    bunch_interp (fill Π Δ) ⊢ bunch_interp (fill Π Δ').
+  Proof.
+    revert Δ Δ'.
+    induction Π as [|C Π IH]=> Δ Δ' H1; eauto.
+    simpl. apply IH.
+    by apply bunch_interp_fill_item_mono.
+  Qed.
+
+  Lemma bunch_ctx_interp_exist Π {I} (P : I → PROP) :
+    bunch_ctx_interp Π (∃ (i : I), P i : PROP)%I ≡
+                     (∃ i, bunch_ctx_interp Π (P i))%I.
+  Proof.
+    revert P. induction Π as [|F Π]=>P.
+    { simpl. reflexivity. }
+    rewrite bunch_ctx_interp_cons.
+    Opaque bunch_ctx_interp.
+    destruct F as [sp ?|sp ?]; destruct sp; simpl.
+    + rewrite bi.sep_exist_r.
+      apply (IHΠ (λ i, P i ∗ bunch_interp Δ2)%I).
+    + rewrite bi.and_exist_r.
+      apply (IHΠ (λ i, P i ∧ bunch_interp Δ2)%I).
+    + rewrite bi.sep_exist_l.
+      apply (IHΠ (λ i, bunch_interp Δ1 ∗ P i)%I).
+    + rewrite bi.and_exist_l.
+      apply (IHΠ (λ i, bunch_interp Δ1 ∧ P i)%I).
+  Qed.
+
+  Global Instance bunch_interp_proper : Proper ((≡) ==> (≡)) bunch_interp.
+  Proof.
+    intros Δ1 Δ2. induction 1; eauto.
+    - etrans; eassumption.
+    - apply bi.equiv_entails_2.
+      + apply bunch_interp_fill_mono; eauto.
+        by apply bi.equiv_entails_1_1.
+      + apply bunch_interp_fill_mono; eauto.
+        by apply bi.equiv_entails_1_2.
+    - simpl. destruct s; by rewrite left_id.
+    - simpl. destruct s; by rewrite comm.
+    - simpl. destruct s; by rewrite assoc.
+  Qed.
+
+  Global Instance bunch_ctx_interp_mono Π : Proper ((⊢) ==> (⊢)) (bunch_ctx_interp Π).
+  Proof.
+    induction Π as [|F Π]=>P1 P2 HP; first by simpl; auto.
+    rewrite !bunch_ctx_interp_cons.
+    apply IHΠ.
+    destruct F as [[|] ? | [|] ?]; simpl; f_equiv; eauto.
+  Qed.
+
+End interp.
+
+Arguments sep_interp {_} _ _ _.
+Arguments bunch_interp {_ _} _ _.
+
