theories/s4/formula.v
@@ -1,0 +1,52 @@
+From Coq Require Import ssreflect.
+From stdpp Require Import prelude gmap fin_sets.
+From bunched.algebra Require Import bi.
+From bunched Require Import bunches.
+
+(** * Formulas *)
+Definition atom := nat.
+
+(** ** Formulas and bunches *)
+Inductive formula : Type :=
+| TOP
+| EMP
+| BOT
+| ATOM (A : atom)
+| CONJ (ϕ ψ : formula)
+| DISJ (ϕ ψ : formula)
+| SEP (ϕ ψ : formula)
+| IMPL (ϕ ψ : formula)
+| WAND (ϕ ψ : formula)
+| BOX (ϕ : formula)
+.
+
+(** "Collapse" internalizes the bunch as a formula. *)
+Fixpoint collapse (Δ : @bunch formula) : formula :=
+  match Δ with
+  | frml ϕ => ϕ
+  | ∅ₐ => TOP
+  | ∅ₘ => EMP
+  | Δ ,, Δ' => SEP (collapse Δ) (collapse Δ')
+  | Δ ;, Δ' => CONJ (collapse Δ) (collapse Δ')
+  end%B.
+
+Inductive collapse_gr : @bunch formula → formula → Prop :=
+| collapse_frml ϕ : collapse_gr (frml ϕ) ϕ
+| collapse_top : collapse_gr ∅ₐ%B TOP
+| collapse_emp : collapse_gr ∅ₘ%B EMP
+| collapse_sep Δ1 Δ2 ϕ1 ϕ2 :
+  collapse_gr Δ1 ϕ1 →
+  collapse_gr Δ2 ϕ2 →
+  collapse_gr (Δ1 ,, Δ2)%B (SEP ϕ1 ϕ2)
+| collapse_conj Δ1 Δ2 ϕ1 ϕ2 :
+  collapse_gr Δ1 ϕ1 →
+  collapse_gr Δ2 ϕ2 →
+  collapse_gr (Δ1 ;, Δ2)%B (CONJ ϕ1 ϕ2)
+.
+
+Lemma collapse_gr_sound Δ : collapse_gr Δ (collapse Δ).
+Proof. induction Δ; simpl; try destruct s; try by econstructor. Qed.
+
+Lemma collapse_gr_complete Δ ϕ : collapse_gr Δ ϕ → collapse Δ = ϕ.
+Proof. induction 1; simpl; subst; eauto. Qed.
+
