theories/s4/seqcalc.v
@@ -1,0 +1,152 @@
+(** BI + □ *)
+From Coq Require Import ssreflect.
+From stdpp Require Import prelude.
+From bunched.algebra Require Import bi.
+From bunched Require Export bunches bunch_decomp.
+From bunched.s4 Require Import formula.
+
+Declare Scope bunch_scope.
+Delimit Scope bunch_scope with B.
+
+(** ** Sequent calculus itself *)
+Reserved Notation "P ⊢ᴮ Q" (at level 99, Q at level 200, right associativity).
+Inductive proves : bunch → formula → Prop :=
+(* structural *)
+| BI_Axiom (a : atom) : frml (ATOM a) ⊢ᴮ ATOM a
+| BI_Equiv Δ Δ' ϕ :
+    (Δ ≡ Δ') → (Δ ⊢ᴮ ϕ) →
+    Δ' ⊢ᴮ ϕ
+| BI_Weaken C Δ Δ' ϕ : (fill C Δ ⊢ᴮ ϕ) →
+                       fill C (Δ ;, Δ') ⊢ᴮ ϕ
+| BI_Contr C Δ ϕ : (fill C (Δ ;, Δ) ⊢ᴮ ϕ) →
+                   fill C Δ ⊢ᴮ ϕ
+(* modalities *)
+| BI_Box_L Π ϕ ψ :
+    (fill Π (frml ϕ) ⊢ᴮ ψ) →
+    fill Π (frml (BOX ϕ)) ⊢ᴮ ψ
+| BI_Box_R Δ ϕ :
+    (BOX <$> Δ ⊢ᴮ ϕ) →
+    BOX <$> Δ ⊢ᴮ BOX ϕ
+(* multiplicatives *)
+| BI_Emp_R :
+    ∅ₘ ⊢ᴮ EMP
+| BI_Emp_L C ϕ :
+    (fill C ∅ₘ ⊢ᴮ ϕ) →
+    fill C (frml EMP) ⊢ᴮ ϕ
+| BI_Sep_R Δ Δ' ϕ ψ :
+    (Δ ⊢ᴮ ϕ) →
+    (Δ' ⊢ᴮ ψ) →
+    Δ ,, Δ' ⊢ᴮ SEP ϕ ψ
+| BI_Sep_L C ϕ ψ χ :
+    (fill C (frml ϕ ,, frml ψ) ⊢ᴮ χ) →
+    fill C (frml (SEP ϕ ψ)) ⊢ᴮ χ
+| BI_Wand_R Δ ϕ ψ :
+    (Δ ,, frml ϕ ⊢ᴮ ψ) →
+    Δ  ⊢ᴮ WAND ϕ ψ
+| BI_Wand_L C Δ ϕ ψ χ :
+    (Δ ⊢ᴮ ϕ) →
+    (fill C (frml ψ) ⊢ᴮ χ) →
+    fill C (Δ ,, frml (WAND ϕ ψ)) ⊢ᴮ χ
+(* additives *)
+| BI_False_L C ϕ :
+    fill C (frml BOT) ⊢ᴮ ϕ
+| BI_True_R Δ :
+    Δ ⊢ᴮ TOP
+| BI_True_L C ϕ :
+    (fill C ∅ₐ ⊢ᴮ ϕ) →
+    fill C (frml TOP) ⊢ᴮ ϕ
+| BI_Conj_R Δ Δ' ϕ ψ :
+    (Δ ⊢ᴮ ϕ) →
+    (Δ' ⊢ᴮ ψ) →
+    Δ ;, Δ' ⊢ᴮ CONJ ϕ ψ
+| BI_Conj_L C ϕ ψ χ :
+    (fill C (frml ϕ ;, frml ψ) ⊢ᴮ χ) →
+    fill C (frml (CONJ ϕ ψ)) ⊢ᴮ χ
+| BI_Disj_R1 Δ ϕ ψ :
+    (Δ ⊢ᴮ ϕ) →
+    Δ ⊢ᴮ DISJ ϕ ψ
+| BI_Disj_R2 Δ ϕ ψ :
+    (Δ ⊢ᴮ ψ) →
+    Δ ⊢ᴮ DISJ ϕ ψ
+| BI_Disj_L Π ϕ ψ χ :
+    (fill Π (frml ϕ) ⊢ᴮ χ) →
+    (fill Π (frml ψ) ⊢ᴮ χ) →
+    fill Π (frml (DISJ ϕ ψ)) ⊢ᴮ χ
+| BI_Impl_R Δ ϕ ψ :
+    (Δ ;, frml ϕ ⊢ᴮ ψ) →
+    Δ  ⊢ᴮ IMPL ϕ ψ
+| BI_Impl_L C Δ ϕ ψ χ :
+    (Δ ⊢ᴮ ϕ) →
+    (fill C (frml ψ) ⊢ᴮ χ) →
+    fill C (Δ ;, frml (IMPL ϕ ψ)) ⊢ᴮ χ
+where "Δ ⊢ᴮ ϕ" := (proves Δ%B ϕ%B).
+
+
+Global Instance proves_proper : Proper ((≡) ==> (=) ==> (≡)) proves.
+Proof.
+  intros D1 D2 HD ϕ ? <-.
+  split; intros H.
+  - eapply BI_Equiv; eauto.
+  - eapply BI_Equiv; [ symmetry | ]; eauto.
+Qed.
+
+(** Additional lemmas for bunch_decompose and box *)
+Lemma bunch_decomp_box_frml Π ϕ Δ :
+  bunch_decomp (BOX <$> Δ) Π (frml ϕ) → ∃ ψ, ϕ = BOX ψ.
+Proof.
+  revert Π. induction Δ=>/= Π H1; try by inversion H1.
+  - inversion H1; simplify_eq/=. naive_solver.
+  - inversion H1 as [Δ|sp Δ1' Δ2' Π' Δ H1' |sp Δ1' Δ2' Π' Δ H1']; simplify_eq/=.
+    + eapply IHΔ1; eauto.
+    + eapply IHΔ2; eauto.
+Qed.
+
+Lemma bunch_decomp_box Δ Π ϕ :
+  bunch_decomp (BOX <$> Δ) Π (frml (BOX ϕ)) →
+  ∃ Π', Π = bunch_ctx_map BOX Π' ∧ bunch_decomp Δ Π' (frml ϕ).
+Proof.
+  revert Π. induction Δ=>/= Π H1; try by inversion H1.
+  - inversion H1. simplify_eq/=. exists []. split; eauto.
+    econstructor.
+  - inversion H1 as [Δ|sp Δ1' Δ2' Π' Δ H1' |sp Δ1' Δ2' Π' Δ H1']; simplify_eq/=.
+    + destruct (IHΔ1 _ H1') as (Π'1 & -> & Hdec).
+      exists (Π'1 ++ [CtxL s Δ2]).
+      rewrite /bunch_ctx_map map_app /=. split; auto.
+        by econstructor.
+    + destruct (IHΔ2 _ H1') as (Π'1 & -> & Hdec).
+      exists (Π'1 ++ [CtxR s Δ1]).
+      rewrite /bunch_ctx_map map_app /=. split; auto.
+        by econstructor.
+Qed.
+
+(** Some convenient derived rules *)
+Lemma BI_Boxes_L Π Δ ϕ :
+  (fill Π Δ ⊢ᴮ ϕ) →
+  (fill Π (BOX <$> Δ) ⊢ᴮ ϕ).
+Proof.
+  revert Π. induction Δ=> Π IH /=; eauto.
+  - by apply BI_Box_L.
+  - apply (IHΔ1 ((CtxL s (fmap BOX Δ2))::Π)). simpl.
+    apply (IHΔ2 ((CtxR s Δ1)::Π)). done.
+Qed.
+
+Lemma BI_Collapse_L Π Δ ϕ :
+  (fill Π Δ ⊢ᴮ ϕ) →
+  (fill Π (frml (collapse Δ)) ⊢ᴮ ϕ).
+Proof.
+  revert Π. induction Δ=>Π; simpl; eauto.
+  - intros HX.
+    destruct s.
+    + by apply BI_Emp_L, HX.
+    + by apply BI_True_L, HX.
+  - intros HX.
+    destruct s.
+    + apply BI_Sep_L.
+      apply (IHΔ1 (CtxCommaL _::Π)); simpl.
+      apply (IHΔ2 (CtxCommaR _::Π)); simpl.
+      apply HX.
+    + apply BI_Conj_L.
+      apply (IHΔ1 (CtxSemicL _::Π)); simpl.
+      apply (IHΔ2 (CtxSemicR _::Π)); simpl.
+      apply HX.
+Qed.
